about to do something dramatic with BlockCache

disk-betree/BlockCache.dfy
@@ -1,17 +1,21 @@
 abstract module BlockCache {
-  type Reference(==)
-
   type Constants
   type Variables(!new)<T>
 
-  function Read<T>(k: Constants, s: Variables, ref: Reference) : T
+  type Reference(!new,==)
 
-  datatype
-    CacheOp<T> = AllocOp(block: T, successors: iset<Reference>, new_ref: Reference)
+  function View<T>(k: Constants, s: Variables) : imap<Reference, T>
+    ensures forall ref :: ref in View(k, s)
+    
+  function Read<T>(k: Constants, s: Variables, ref: Reference) : T
+    ensures Read(k, s, ref) == View(k, s)[ref];
+    
+  datatype CacheOp<T> =
+    | AllocOp(block: T, successors: iset<Reference>, new_ref: Reference)
     | WriteOp(ref: Reference, block: T, successors: iset<Reference>)
     
   predicate Apply(k: Constants, s: Variables, s': Variables, op: CacheOp)
-      
+    
   predicate Apply2(k: Constants, s: Variables, s': Variables, op1: CacheOp, op2: CacheOp) {
     exists sint :: 
       && Apply(k, s, sint, op1)
